process/typecheck.v
@@ -1,117 +1,115 @@
 From SST Require Import aux.unscoped aux.expressions process.processes type.global tree.global tree.local.
-Require Import List String Datatypes ZArith Relations.
+Require Import List String Datatypes ZArith Relations PeanoNat.
 Open Scope list_scope.
 From mathcomp Require Import ssreflect.seq.
 Import ListNotations.
 From Paco Require Import paco.
 
-Inductive ctx: Type :=
-  | empty: ctx
-  | consS: fin -> sort -> ctx -> ctx
-  | consT: fin -> ltt -> ctx -> ctx.
+Inductive ctxS : Type := 
+  | emptyS : ctxS
+  | consS : fin -> sort -> ctxS -> ctxS.
 
-Fixpoint memS (n: fin) (s: sort) (m: ctx): Prop :=
+Inductive ctxT : Type := 
+  | emptyT : ctxT 
+  | consT : fin -> ltt -> ctxT -> ctxT.
+
+(* Fixpoint memS (n: fin) (s: sort) (m: ctxS): Prop :=
   match m with
     | consS u v m1 => (n = u /\ (subsort s v \/ v = s)) \/ memS n s m1
-    | consT u v m1 => memS n s m1
     | _            => False
   end.
 
-Fixpoint memT (n: fin) (t: ltt) (m: ctx): Prop :=
+Fixpoint memT (n: fin) (t: ltt) (m: ctxT): Prop :=
   match m with
     | consT u v m1 => (n = u /\ (subtypeC t v \/ v = t)) \/ memT n t m1
-    | consS u v m1 => memT n t m1
     | _            => False
-  end.
+  end. *)
 
-Definition extendS (m: ctx) (s: fin) (t: expressions.sort) :=
+Definition extendS (m: ctxS) (s: fin) (t: expressions.sort) :=
   consS s t m.
 
-Definition extendT (m: ctx) (s: fin) (t: ltt) :=
+Definition extendT (m: ctxT) (s: fin) (t: ltt) :=
   consT s t m.
 
-Fixpoint lookupS (m: ctx) (s: fin): option expressions.sort :=
+(* Lookup by shadowing *)
+Fixpoint lookupS (m: ctxS) (s: fin): option expressions.sort :=
   match m with
-    | empty          => None
     | consS s' t' xs => if Nat.eqb s s' then Some t' else lookupS xs s
-    | consT s' t' xs => lookupS xs s
+    | emptyS          => None
   end.
 
-Fixpoint lookupT (m: ctx) (s: fin): option ltt :=
+Fixpoint lookupT (m: ctxT) (s: fin): option ltt :=
   match m with
-    | empty          => None
     | consT s' t' xs => if Nat.eqb s s' then Some t' else lookupT xs s
-    | consS s' t' xs => lookupT xs s
+    | emptyT          => None
   end.
 
-Fixpoint infr_expr (m: ctx) (e: expr): option sort :=
-  match e with
-    | e_var x   => lookupS m x
-    | e_val v   => 
-      match v with
-        | vint i  => Some sint
-        | vbool b => Some sbool
-        | vunit u => Some sunit
-        | vnat n =>  Some snat
-      end
-    | e_succ e1 => 
-      let se1 := infr_expr m e1 in
-      match se1 with
-        | Some gint => Some sint
-        | _         => None
-      end
-    | e_neg e1 => 
-      let se1 := infr_expr m e1 in
-      match se1 with
-        | Some gint => Some sint
-        | _         => None
-      end
-    | e_not e1 => 
-      let se1 := infr_expr m e1 in
-      match se1 with
-        | Some goobl => Some sbool
-        | _          => None
-      end
-    | e_gt e1 e2 => 
-      let se1 := infr_expr m e1 in
-      let se2 := infr_expr m e2 in
-      match pair se1 se2 with
-        | pair (Some sint) (Some sint) => Some sbool
-        | _                            => None
-      end
-    | e_plus e1 e2 => 
-      let se1 := infr_expr m e1 in
-      let se2 := infr_expr m e2 in
-      match pair se1 se2 with
-        | pair (Some sint) (Some sint) => Some sint
-        | _                            => None
+Inductive subCtxS : ctxS -> ctxS -> Prop := 
+  | sctxs_app : forall m s s' c c', subCtxS c c' -> subsort s s' -> subCtxS (consS m s c) (consS m s' c') 
+  | sctxs_appe: forall m s c c', subCtxS c c' -> subCtxS (consS m s c) (consS m s c') 
+  | sctxs_ref : forall c, subCtxS c c.
+
+Inductive subCtxT : ctxT -> ctxT -> Prop := 
+  | sctxt_app : forall m t t' c c', subCtxT c c' -> subtypeC t t' -> subCtxT (consT m t c) (consT m t' c')
+  | sctxt_appe: forall m t c c', subCtxT c c' -> subCtxT (consT m t c) (consT m t c') 
+  | sctxt_ref : forall c, subCtxT c c.
+
+Fixpoint refCtxS (c1 c2: ctxS) : Prop := 
+  match (c1, c2) with 
+    | (consS u1 v1 m1, consS u2 v2 m2) => (u1 = u2 /\ (subsort v1 v2 \/ v1 = v2) /\ refCtxS m1 m2)
+    | (emptyS, emptyS) => True
+    | _ => False
+  end.
+  
+Fixpoint refCtxT (c1 c2: ctxT) : Prop := 
+  match (c1, c2) with 
+    | (consT u1 v1 m1, consT u2 v2 m2) => (u1 = u2 /\ (subtypeC v1 v2 \/ v1 = v2) /\ refCtxT m1 m2)
+    | (emptyT, emptyT) => True
+    | _ => False
+  end.
+
+(* Definition eq_ctxS (m1 m2 : ctxS) := forall n s, memS n s m1 <-> memS n s m2.
+  
+Definition eq_ctxT (m1 m2 : ctxT) := forall n t, memT n t m1 <-> memT n t m2.
+
+Definition leq_ctxS (m1 m2 : ctxS) := forall n s, memS n s m1 -> memS n s m2.
+  
+Definition leq_ctxT (m1 m2 : ctxT) := forall n t, memT n t m1 -> memT n t m2. *)
+
+Definition leq_sinctx_prop (n : fin) (m1 m2 : ctxS) : Prop :=
+  match lookupS m1 n with
+    | Some s => match lookupS m2 n with
+        | Some s' => subsort s s' 
+        | None => False 
+       end
+    | None => match lookupS m2 n with
+        | Some s' => False
+        | None => True
       end
   end.
 
-Inductive subCtx: ctx -> ctx -> Prop :=
-  | sctx1: forall m t t' c c', subCtx c c' -> subtypeC t t' -> subCtx (consT m t c) (consT m t' c')
-  | sctx2: forall m t c c', subCtx c c' -> subCtx (consT m t c) (consT m t c')
-  | sctx3: forall m s s' c c', subCtx c c' -> subsort s s' -> subCtx (consS m s c) (consS m s' c')
-  | sctx4: forall m s c c', subCtx c c' -> subCtx (consS m s c) (consS m s c')
-  | subctxr: forall c, subCtx c c. 
-
-Fixpoint refCtxT (c1 c2: ctx): Prop :=
-  match (c1, c2) with
-    | (consT u1 v1 m1, consT u2 v2 m2) => (u1 = u2 /\ (subtypeC v1 v2 \/ v1 = v2)) /\ refCtxT m1 m2
-    | (consS u1 v1 m1, consS u2 v2 m2) => (u1 = u2 /\ (subsort  v1 v2 \/ v1 = v2)) /\ refCtxT m1 m2
-    | (empty, empty)                   => True
-    | _                                => False
+Definition leq_tinctx_prop (n : fin) (m1 m2 : ctxT) : Prop := 
+  match lookupT m1 n with 
+    | Some t => match lookupT m2 n with
+        | Some t' => subtypeC t t'
+        | None => False 
+       end
+    | None => match lookupT m2 n with
+        | Some t' => False
+        | None => True 
+       end
   end.
 
-Definition eq_ctx (m1 m2: ctx) := 
-  (forall n s, memS n s m1 <-> memS n s m2) /\
-  (forall n t, memT n t m1 <-> memT n t m2).
+Definition eq_ctxS (m1 m2 : ctxS) := forall n, (leq_sinctx_prop n m1 m2) /\ (leq_sinctx_prop n m2 m1).
+  
+Definition eq_ctxT (m1 m2 : ctxT) := forall n, (leq_tinctx_prop n m1 m2) /\ (leq_tinctx_prop n m2 m1).
 
-Definition eq_ctxL (m1 m2: ctx) := 
-  (forall n s, memS n s m1 -> memS n s m2) /\
-  (forall n t, memT n t m1 -> memT n t m2).
+Definition leq_ctxS (m1 m2 : ctxS) := forall n, (leq_sinctx_prop n m1 m2).
+  
+Definition leq_ctxT (m1 m2 : ctxT) := forall n, (leq_tinctx_prop n m1 m2).
 
-Inductive typ_expr: ctx -> expr -> sort -> Prop :=
+
+Inductive typ_expr: ctxS -> expr -> sort -> Prop :=
   | sc_var : forall c s t, Some t = lookupS c s -> typ_expr c (e_var s) t
   | sc_vali: forall c i, typ_expr c (e_val (vint i)) sint
   | sc_valn: forall c i, typ_expr c (e_val (vnat i)) snat
@@ -122,7 +120,7 @@ Inductive typ_expr: ctx -> expr -> sort -> Prop :=
                          typ_expr c (e_neg e) sint
   | sc_sub : forall c c' e s s', typ_expr c e s ->
                                  subsort s s' ->
-                                 refCtxT c c' ->
+                                 leq_ctxS c c' ->
                                  typ_expr c' e s'
   | sc_not : forall c e, typ_expr c e sbool ->
                          typ_expr c (e_not e) sbool
@@ -147,120 +145,177 @@ Fixpoint matchSel (l: label) (xs: list(label*(expressions.sort)*ltt)%type): opti
 
 Definition IF_then_else (P Q R:Prop) := P /\ Q \/ ~ P /\ R.
 
-Fixpoint findCtx (n: fin) (t: ltt) (m: ctx): Prop :=
+Fixpoint findCtxT (n: fin) (t: ltt) (m: ctxT): Prop :=
   match m with
-    | consT u v m1 => (n = u /\ v = t) \/ findCtx n t m1
-    | consS u v m1 => findCtx n t m1
+    | consT u v m1 => (n = u /\ v = t) \/ findCtxT n t m1
     | _            => False
   end.
 
-Inductive typ_proc: fin -> fin -> ctx -> process -> ltt -> Prop :=
-  | tc_inact: forall m em c, typ_proc m em c (p_inact) (ltt_end)
-  | tc_var  : forall m em c s t, Some t = lookupT c s ->
-                                 typ_proc m em c (p_var s) t
-  | tc_mu   : forall m em c p t, let c' := extendT c m t in
-                                 typ_proc (S m) em c' p t ->
-                                 typ_proc m em c (p_rec p) t
-  | tc_ite  : forall m em c e p1 p2 T, typ_expr c e sbool ->
-                                       typ_proc m em c p1 T ->
-                                       typ_proc m em c p2 T ->
-                                       typ_proc m em c (p_ite e p1 p2) T
-  | tc_sub  : forall m em c c' p t t', typ_proc m em c p t ->
-                                       subtypeC t t' ->
-                                       refCtxT c c' -> 
-                                       typ_proc m em c' p t'
-  | tc_recv : forall m em c p L ST P T,
+Inductive typ_proc: fin -> ctxS -> ctxT -> process -> ltt -> Prop :=
+  | tc_inact: forall em cs ct, typ_proc em cs ct (p_inact) (ltt_end)
+  | tc_var  : forall em cs ct s t, Some t = lookupT ct s ->
+                                   typ_proc em cs ct (p_var s) t
+  | tc_mu   : forall em cs ct x p t, let ct' := extendT ct x t in
+                                     typ_proc em cs ct' p t ->
+                                     typ_proc em cs ct (p_rec x p) t
+  | tc_ite  : forall em cs ct e p1 p2 T, typ_expr cs e sbool ->
+                                         typ_proc em cs ct p1 T ->
+                                         typ_proc em cs ct p2 T ->
+                                         typ_proc em cs ct (p_ite e p1 p2) T
+  | tc_sub  : forall em cs cs' ct ct' p t t', typ_proc em cs ct p t ->
+                                              subtypeC t t' ->
+                                              leq_ctxS cs cs' ->
+                                              leq_ctxT ct ct' -> 
+                                              typ_proc em cs' ct' p t'
+  | tc_recv : forall em cs ct p L ST P T,
                      length L = length ST ->
                      length ST = length P ->
                      length P = length T ->
-                     List.Forall (fun u => typ_proc m (S em) (extendS c em (fst u)) (fst (snd u)) (snd (snd u))) (zip ST (zip P T)) ->
-                     typ_proc m em c (p_recv p (zip (zip L ST) P)) (ltt_recv p (zip (zip L ST) T))
-  | tc_send: forall m em c p l e P S T, typ_expr c e S ->
-                                        typ_proc m em c P T ->
-                                        typ_proc m em c (p_send p l e P) (ltt_send p [(l,S,T)]).
+                     List.Forall (fun u => typ_proc (S em) (extendS cs em (fst u)) ct (fst (snd u)) (snd (snd u))) (zip ST (zip P T)) ->
+                     typ_proc em cs ct (p_recv p (zip L P)) (ltt_recv p (zip (zip L ST) T))
+  | tc_send: forall em cs ct p l e P S T, typ_expr cs e S ->
+                                          typ_proc em cs ct P T ->
+                                          typ_proc em cs ct (p_send p l e P) (ltt_send p [(l,S,T)]).
 
-
-Lemma _a23_d: forall P m em Q T G,
-  typ_proc m em G P T ->
-  (P = (p_rec Q) -> typ_proc (S m) em (extendT G m T) Q T).
-Proof. intros.
-       induction H; intros; try easy.
-       inversion H0.
-       subst.
-(*        destruct H0 as (Ha, Hb). *)
-(*        inversion Ha. subst.  *)
-       unfold c' in *.
-       easy.
-
-       specialize(tc_sub (S m) em (extendT c m t) (extendT c' m t') Q t t'); intro Hs.
-       apply Hs.
-       apply IHtyp_proc. easy. easy.
-       simpl.
-       split. split. easy.
-       left. easy.
-       easy.
+Lemma natb_to_prop : forall a b, (a =? b)%nat = true -> a = b.
+Proof. 
+    intros a b.
+    specialize(Nat.eqb_eq a b); intro H1.
+    destruct H1.
+    easy.
 Qed.
 
-Definition PBob: process := p_recv "Alice" [(1, snat, p_send "Carol" 2 (e_val (vnat 100)) p_inact);
-                                            (4, snat, p_send "Carol" 2 (e_val (vnat 2)) p_inact)].
+Lemma natb_to_propf : forall a b, (a =? b)%nat = false -> a <> b.
+Proof.
+    intros a b.
+    specialize(Nat.eqb_neq a b); intro H1.
+    destruct H1.
+    easy.
+Qed.
+(* 
+Lemma ref_stronger_C : forall cs cs', refCtxS cs cs' -> leq_ctxS cs cs'. 
+  intros cs cs'.
+  induction 
+  destruct cs, cs'. easy. easy. easy.
+  induction cs. 
+  induction cs'. 
+  easy. easy.
+  intros.
+  
+  
+  induction cs'.
+  
+    
+  induction cs'.
+  easy.
+  intros.
+  simpl in H.
+  simpl in IHcs, IHcs'.
+  
+  
+  unfold refCtxS in *.  
+  
 
-Definition TBob: ltt := ltt_recv "Alice" [(1, snat, ltt_send "Carol" [(2, snat, ltt_end)]);
-                                          (4, snat, ltt_send "Carol" [(2, snat, ltt_end)])].
 
-Example _317_b: typ_proc 0 0 empty PBob TBob.
-Proof. unfold PBob, TBob.
-       (* typechecking the outermost structure *)
-       specialize(tc_recv 0 0 empty "Alice"
-                         [1; 4]
-                         [snat; snat]
-                         [(p_send "Carol" 2 (e_val (vnat 100)) p_inact); (p_send "Carol" 2 (e_val (vnat 2)) p_inact)]
-                         [(ltt_send "Carol" [(2, snat, ltt_end)]); (ltt_send "Carol" [(2, snat, ltt_end)])]
-                         ); intro HR.
-       simpl in HR.
-       apply HR; clear HR; try easy.
-       apply Forall_forall.
-       intros (s, (p, l)) HIn.
-       simpl in HIn.
-       destruct HIn as [HIn | HIn].
-       inversion HIn. simpl.
-       subst.
+Admitted.
 
-       (* typechecking the first continuation *)
-       specialize(tc_send 0 1 (extendS empty 0 snat) "Carol"
-                          2
-                          (e_val (vnat 100))
-                          p_inact
-                          snat
-                          ltt_end
-         ); intro HS.
-       simpl in HS.
-       apply HS; clear HS.
+Lemma ref_stronger_T : forall ct ct', refCtxT ct ct' -> leq_ctxT ct ct'. 
+Admitted. *)
 
-       (*expression typcheck*)
-       constructor.
+Lemma leq_ctxS_refl : forall cs, leq_ctxS cs cs.
+Proof.
+  intros. unfold leq_ctxS.
+  intros. unfold leq_sinctx_prop.
+  destruct lookupS. 
+  apply (srefl s).
+  easy. 
+Qed.
 
-       constructor.
-       simpl.
-       destruct HIn as [HIn | HIn].
-       inversion HIn. simpl.
-       subst.
-       (* typechecking the second continuation *)
-       specialize(tc_send 0 1 (extendS empty 0 snat) "Carol"
-                          2
-                          (e_val (vnat 2))
-                          p_inact
-                          snat
-                          ltt_end
-         ); intro HS.
-       simpl in HS.
-       apply HS; clear HS.
+Lemma leq_ctxT_refl : forall ct, leq_ctxT ct ct.
+Proof.
+  intros. unfold leq_ctxT.
+  intros. unfold leq_tinctx_prop.
+  destruct lookupT. easy. easy.
+Qed.
 
-       (*expression typcheck*)
-       constructor.
+Lemma leq_ctxC_trans : forall cs1 cs2 cs3, leq_ctxS cs1 cs2 -> leq_ctxS cs2 cs3 -> leq_ctxS cs1 cs3.
+Proof.
+  intros.
+  unfold leq_ctxS in *.
+  unfold leq_sinctx_prop in *.
+  intro n.
+  specialize(H n); intros.
+  specialize(H0 n); intros.
+  induction cs1; intros; try easy.
+  simpl.
+  simpl in H.
+  induction cs2; intros; try easy.
+  case_eq (Nat.eqb n n0); intros.
+  specialize(natb_to_prop n n0 H1); intros. subst. simpl in H.
+  replace ((n0 =? n0)%nat) with true in H. 
+  contradiction.
+  simpl in H.
+  replace ((n =? n0)%nat) with false in H.
+  specialize(IHcs2 H); intros.
+  simpl in H0. 
+  replace ((n =? n0)%nat) with false in H0.
+  specialize(IHcs2 H0); intros. 
+  easy.
+  
+  simpl.
+  case_eq (Nat.eqb n n0); intros.
+  simpl in H.
+  replace ((n =? n0)%nat) with true in H.
+  
+  
+  destruct (lookupS cs2 n) in *. 
+  destruct (lookupS cs3 n) in *.
+  specialize(sstrans s s0 s1 H H0); intros. 
+  easy. easy.
+  contradiction.
+  simpl in H.
+  replace ((n =? n0)%nat) with false in H.
+  specialize(IHcs1 H); intros. easy.
+Qed.
 
-       constructor.
-
-       easy.
+Lemma leq_ctxT_trans : forall ct1 ct2 ct3, leq_ctxT ct1 ct2 -> leq_ctxT ct2 ct3 -> leq_ctxT ct1 ct3.
+Proof.
+  intros.
+  unfold leq_ctxT in *.
+  unfold leq_tinctx_prop in *.
+  intro n.
+  specialize(H n); intros.
+  specialize(H0 n); intros.
+  induction ct1; intros; try easy.
+  simpl.
+  simpl in H.
+  induction ct2; intros; try easy.
+  case_eq (Nat.eqb n n0); intros.
+  specialize(natb_to_prop n n0 H1); intros. subst. simpl in H.
+  replace ((n0 =? n0)%nat) with true in H. 
+  contradiction.
+  simpl in H.
+  replace ((n =? n0)%nat) with false in H.
+  specialize(IHct2 H); intros.
+  simpl in H0. 
+  replace ((n =? n0)%nat) with false in H0.
+  specialize(IHct2 H0); intros. 
+  easy.
+  
+  simpl.
+  case_eq (Nat.eqb n n0); intros.
+  simpl in H.
+  replace ((n =? n0)%nat) with true in H.
+  
+  
+  destruct (lookupT ct2 n) in *. 
+  destruct (lookupT ct3 n) in *.
+  specialize(stTrans l l0 l1 H H0); intros. 
+  easy. easy.
+  contradiction.
+  simpl in H.
+  replace ((n =? n0)%nat) with false in H.
+  specialize(IHct1 H); intros. easy.
 Qed.
 
 Lemma empty_nil: forall {A: Type} (l: list A),
@@ -269,53 +324,9 @@ Proof. intros A l.
        case l; intros; easy.
 Qed.
 
-Lemma zip_eq: forall {A B: Type} (l1 l3: list A) (l2 l4: list B),
-  length l1 = length l2 -> length l2 = length l3 -> length l3 = length l4 ->
-  (zip l1 l2) = (zip l3 l4) ->
-  l1 = l3 /\ l2 = l4.
-Proof. intros A B l1.
-       induction l1; intros.
-       - simpl in *.
-         rewrite <- H in H0.
-         rewrite <- H0 in H1.
-         rewrite empty_nil in H.
-         rewrite empty_nil in H0.
-         rewrite empty_nil in H1.
-         subst. easy.
-       - simpl in H.
-         case_eq l2; intros.
-         + subst. simpl in *. easy.
-         + subst. simpl in *.
-           case_eq l3; intros.
-           ++ subst. easy.
-           ++ case_eq l4; intros.
-              -- subst. easy.
-              -- subst. simpl in *.
-                 inversion H2. subst.
-                 inversion H.
-                 inversion H1.
-                 inversion H0.
-                 specialize(IHl1 l0 l l2 H4 H7 H5 H6).
-                 split. f_equal. easy.
-                 f_equal. easy.
-Qed.
 
-Lemma zip_len: forall {A B: Type} (l1: list A) (l2: list B),
-  length l1 = length l2 -> length l1 = length (zip l1 l2).
-Proof. intros A B l1.
-       induction l1; intros.
-       - simpl in H. rewrite empty_nil in H.
-         subst. simpl. easy.
-       - simpl in H. simpl.
-         case_eq l2; intros.
-         subst. easy.
-         subst. simpl in H.
-         inversion H.
-         simpl. f_equal.
-         apply IHl1. easy.
-Qed.
-
-(* Lemma ref_ctx_1: forall c c' t t' u,
+(* 
+Lemma ref_ctx_1: forall c c' t t' u,
  refCtxT t t' c c' -> refCtxT u u c c'.
 Proof. intro c.
        induction c; intros.
@@ -340,8 +351,8 @@ Proof. intro c.
            subst.
            
            subst. split. easy. split. easy.
-           apply IHc with (t := t) (t' := t'). easy. *)
-
+           apply IHc with (t := t) (t' := t'). easy. 
+(*  *)
 Example complex_mu : process := 
   p_rec (p_recv "Alice" [
     (0, sbool, p_var 0);
@@ -353,562 +364,15 @@ Example complex_mu : process :=
     (2, sbool, p_inact)
   ]).
 
-Compute unfold_rec complex_mu.
-
-
-Lemma _a23_a: forall m em p L S Q P G T, 
-  typ_proc m em G P T ->
-  P = (p_recv p (zip (zip L S) Q)) -> 
-  (exists T', length T' = length L -> length T' = length S -> length T' = length Q -> subtypeC (ltt_recv p (zip (zip L S) T')) T /\  
-  List.Forall (fun u => typ_proc m (Datatypes.S em) (extendS G em (fst u)) (fst (snd u)) (snd (snd u))) (zip S (zip Q T'))).
-Proof. intros.
-       induction H; intros; try easy.
-       specialize(IHtyp_proc H0).
-       destruct IHtyp_proc as (T',IHtyp_proc).
-       exists T'. intros Hla1 Hla2 Hla3.
-       split.
-       specialize(IHtyp_proc Hla1 Hla2 Hla3).
-       destruct IHtyp_proc as (IHtyp_proc, Ha).
-       specialize(stTrans (ltt_recv p (zip (zip L S) T')) t t' IHtyp_proc); intro HT.
-       apply HT.
-       
-        easy.
-       
-       (**)
-       destruct IHtyp_proc as (IHtyp_proc, Ha). easy. easy. easy.
-       apply Forall_forall.
-       intros (x1,(x2,x3)) Hx.
-       simpl in *.
-       rewrite Forall_forall in Ha.
-       specialize(Ha (x1,(x2,x3))). simpl in Ha.
-       specialize(tc_sub m (Datatypes.S em) (extendS c em x1) (extendS c' em x1) x2 x3 x3); intro HTC.
-       apply HTC.
-(*        specialize(tc_sub m (Datatypes.S em) c); intro HTC. *)
-       apply Ha. easy.
-       apply stRefl.
-       simpl.
-       split. split. easy.  right. easy. easy.
-
-       rewrite Forall_forall in H3.
-       exists T.
-       intros Hla1 Hla2 Hla3.
-       split.
-       inversion H0. subst.
-       assert(length (zip L0 ST) = length L0) as Hasrt1.
-       { symmetry.
-         apply zip_len. easy.
-       }
-       assert(L = L0).
-       { specialize(zip_eq (zip L0 ST) (zip L S) P Q); intro HH.
-         assert(length (zip L0 ST) = length P).
-         { symmetry.
-           rewrite <- H1, <- H.
-           apply zip_len. easy.
-         }
-         assert(length P = length (zip L S)).
-         {
-           rewrite H2, Hla1. apply zip_len.
-           rewrite <- Hla1. easy.
-         }
-         assert(length (zip L S) = length Q).
-         {  rewrite <- Hla3, Hla1.
-            symmetry. apply zip_len.
-            rewrite <- Hla1.  easy.
-         }
-         specialize(HH H4 H5 H7 H6).
-         destruct HH as (HHa,HHb).
-         specialize(zip_eq L0 L ST S); intro HH1.
-         subst.
-         assert(length ST = length L).
-         { rewrite H1, <- Hla3. easy. }
-         assert(length L = length S).
-         { rewrite <- Hla1. easy. }
-         specialize(HH1 H H8 H9 HHa). easy.
-       }
-       assert(S = ST).
-       {
-         specialize(zip_eq (zip L0 ST) (zip L S) P Q); intro HH.
-         assert(length (zip L0 ST) = length P).
-         { rewrite Hasrt1, H. easy. }
-         assert(length P = length (zip L S)).
-         { rewrite H2, Hla1. apply zip_len.
-           rewrite <- Hla1. easy.
-         }
-         assert(length (zip L S) = length Q).
-         {  rewrite <- Hla3, Hla1.
-            symmetry. apply zip_len.
-            rewrite <- Hla1.  easy.
-         }
-         specialize(HH H5 H7 H8 H6).
-         destruct HH as (HHa,HHb).
-         specialize(zip_eq L0 L ST S); intro HH1.
-         assert(length ST = length L).
-         { rewrite H1, H2. easy. }
-         assert(length L = length S).
-         { rewrite <- Hla1.  easy. }
-         specialize(HH1 H H9 H10 HHa). easy.
-       }
-       assert(P = Q).
-       {
-         specialize(zip_eq (zip L0 ST) (zip L S) P Q); intro HH.
-         assert(length (zip L0 ST) = length P).
-         { symmetry.
-           rewrite <- H1, <- H.
-           apply zip_len. easy.
-         }
-         assert(length P = length (zip L S)).
-         {
-           rewrite H2, Hla1. apply zip_len.
-           rewrite <- Hla1. easy.
-         }
-         assert(length (zip L S) = length Q).
-         {  rewrite <- Hla3, Hla1.
-            symmetry. apply zip_len.
-            rewrite <- Hla1.  easy.
-         }
-         specialize(HH H7 H8 H9 H6). easy.
-       }
-       subst.
-       pfold.
-       apply sub_in. easy. easy.
-       clear H H1 H2 H3 H6 Hla1 Hla2 Hla3 Hasrt1.
-       apply Forall_forall.
-       intros (x1,x2) Hx.
-       induction ST; intros.
-       simpl in Hx. easy.
-       simpl in Hx.
-       destruct Hx as [Hx | Hx].
-       inversion Hx. subst.
-       simpl. apply srefl.
-       simpl. apply IHST. easy. easy.
-
-       apply Forall_forall.
-       intros (x1,x2) Hx.
-       clear H H1 H2 H3 Hla1 Hla2 Hla3 Hasrt1.
-       induction T; intros.
-       simpl in Hx. easy.
-       simpl in Hx.
-       simpl in IHT.
-       destruct Hx as [Hx | Hx].
-       inversion Hx. subst. simpl.
-       specialize(stRefl x2); intro HT.
-       punfold HT. apply st_mon.
-       simpl. apply IHT. easy.
-       
-       (**)
-       apply Forall_forall.
-       intros (x1,(x2,x3)) Hx.
-       simpl in *.
-       specialize(H3 (x1,(x2,x3))). simpl in H3.
-       inversion H0. subst.
-       apply H3.
-       assert(L = L0).
-       { specialize(zip_eq (zip L0 ST) (zip L S) P Q); intro HH.
-         assert(length (zip L0 ST) = length P).
-         { symmetry.
-           rewrite <- H1, <- H.
-           apply zip_len. easy.
-         }
-         assert(length P = length (zip L S)).
-         {
-           rewrite H2, Hla1. apply zip_len.
-           rewrite <- Hla1. easy.
-         }
-         assert(length (zip L S) = length Q).
-         {  rewrite <- Hla3, Hla1.
-            symmetry. apply zip_len.
-            rewrite <- Hla1.  easy.
-         }
-         specialize(HH H4 H5 H7 H6).
-         destruct HH as (HHa,HHb).
-         specialize(zip_eq L0 L ST S); intro HH1.
-         subst.
-         assert(length ST = length L).
-         { rewrite H1, <- Hla3. easy. }
-         assert(length L = length S).
-         { rewrite <- Hla1. easy. }
-         specialize(HH1 H H8 H9 HHa). easy.
-       }
-       assert(S = ST).
-       {
-         specialize(zip_eq (zip L0 ST) (zip L S) P Q); intro HH.
-         assert(length (zip L0 ST) = length P).
-         { rewrite <- H1, <- H.
-           symmetry. apply zip_len. easy.  }
-         assert(length P = length (zip L S)).
-         { rewrite H2, Hla1. apply zip_len.
-           rewrite <- Hla1. easy.
-         }
-         assert(length (zip L S) = length Q).
-         {  rewrite <- Hla3, Hla1.
-            symmetry. apply zip_len.
-            rewrite <- Hla1.  easy.
-         }
-         specialize(HH H5 H7 H8 H6).
-         destruct HH as (HHa,HHb).
-         specialize(zip_eq L0 L ST S); intro HH1.
-         assert(length ST = length L).
-         { rewrite H1, H2. easy. }
-         assert(length L = length S).
-         { rewrite <- Hla1.  easy. }
-         specialize(HH1 H H9 H10 HHa). easy.
-       }
-       assert(P = Q).
-       {
-         specialize(zip_eq (zip L0 ST) (zip L S) P Q); intro HH.
-         assert(length (zip L0 ST) = length P).
-         { symmetry.
-           rewrite <- H1, <- H.
-           apply zip_len. easy.
-         }
-         assert(length P = length (zip L S)).
-         {
-           rewrite H2, Hla1. apply zip_len.
-           rewrite <- Hla1. easy.
-         }
-         assert(length (zip L S) = length Q).
-         {  rewrite <- Hla3, Hla1.
-            symmetry. apply zip_len.
-            rewrite <- Hla1.  easy.
-         }
-         specialize(HH H7 H8 H9 H6). easy.
-       }
-       subst.
-       easy.
-Qed.
-
-Lemma _a23_b: forall m em p l e Q P G T, 
-  typ_proc m em G P T ->
-  (P = (p_send p l e Q) -> exists S S' T', typ_expr G e S /\ typ_proc m em G Q T' /\ subsort S' S /\ subtypeC (ltt_send p [(l,S',T')]) T).
-Proof. intros m em p l e Q P G T H.
-       induction H; intros; try easy.
-       specialize(IHtyp_proc H2).
-       destruct IHtyp_proc as (S,(S',(T',Ha))).
-       exists S. exists S'. exists T'.
-       split.
-       specialize(sc_sub c c' e S S); intro HSS.
-       apply HSS. easy. apply srefl. easy.
-       split.
-       specialize(tc_sub m em c c' Q T' T'); intro HTS.
-       apply HTS. easy.
-       apply stRefl. easy. split. easy.
-       destruct Ha as (Ha,(Hb,(Hc,Hd))).
-       specialize(stTrans (ltt_send p [(l, S', T')]) t t' Hd H0); intro HT.
-       apply HT.
-       exists S. exists S. exists T.
-       inversion H1. subst.
-       split. easy. split. easy.
-       split. apply srefl. 
-       specialize(sub_out (upaco2 subtype bot2)
-          p [l] [S] [S] [T] [T]
-        ); intros HHa.
-       simpl in HHa.
-       pfold.
-       apply HHa. easy. easy.
-       apply Forall_forall. simpl.
-       intros (s1, s2) Hs. destruct Hs.
-       inversion H2. subst. simpl. apply srefl.
-       easy.
-       apply Forall_forall. simpl.
-       intros (T1, T2) Hs. destruct Hs.
-       inversion H2. subst.
-       simpl. left. pfold.
-       specialize(stRefl T2); intro HT.
-       punfold HT. apply st_mon.
-       easy.
-Qed.
-
-Lemma _a23_c: forall P m em e Q1 Q2 T G,
-  typ_proc m em G P T ->
-  (P = (p_ite e Q1 Q2) -> exists T1 T2, typ_proc m em G Q1 T1 /\ typ_proc m em G Q2 T2 /\ subtypeC T1 T /\ subtypeC T2 T).
-Proof. intros.
-       induction H; intros; try easy.
-       inversion H0.
-       subst.
-       exists T. exists T.
-       split. easy. split. easy. split.
-       specialize(stRefl T); intro HT. easy.
-       specialize(stRefl T); intro HT. easy.
-       specialize(IHtyp_proc H0).
-       destruct IHtyp_proc as (T1,(T2,(Ha,(Hb,(Hc,Hd))))).
-       exists T1. exists T2.
-       split.
-       specialize(tc_sub m em c c' Q1 T1 T1); intro HTS.
-       apply HTS. easy. apply stRefl. easy. 
-       split.
-       specialize(tc_sub m em c c' Q2 T2 T2); intro HTS.
-       apply HTS. easy. apply stRefl. easy. 
-       split.
-       specialize(stTrans T1 t t' Hc H1); intro HT. easy.
-       specialize(stTrans T2 t t' Hd H1); intro HT. easy.
-Qed.
-
-
-(* Lemma _a23_d_v2: forall P m em Q T G,
-  typ_proc m em G P T ->
-  (exists T', (P = (p_rec Q) /\ subtypeC T T') -> typ_proc (S m) em (extendT G m T') Q T').
-Proof. intros.
-       induction H; try (exists ltt_end; easy).
-       exists t.
-       intros (Ha, Hb). 
-       inversion Ha. subst. 
-       unfold c' in *.
-       easy.
-
-       destruct IHtyp_proc as (T', Hp).
-       exists T'.
-       intros (Ha, Hb).
-       apply Hp.
-       split. easy.
-       specialize(stTrans t t' T' H0 Hb); intro HT.
-       exact HT.
-Qed.
+Compute unfold_rec complex_mu. 
  *)
 
-Lemma helper0: forall c d n s, refCtxT c d -> memS n s c -> memS n s d.
-Proof. intro c.
-       induction c; intros.
-       - case_eq d; intros.
-         + subst. simpl in H0. easy.
-         + subst. simpl in H0. easy.
-         + subst. simpl in H0. easy.
-       - case_eq d; intros.
-         + subst. simpl in H. easy.
-         + subst. simpl in H. simpl.
-           simpl in H0.
-           destruct H0.
-           destruct H0.
-           subst. 
-           destruct H1. left.
-           split. easy.
-           destruct H. destruct H. destruct H2.
-           subst. left.
-           apply sstrans with (s2 := s); easy.
-           subst. left. easy.
-           subst. left.
-           destruct H.
-           destruct H. split. easy.
-           destruct H1. left. easy. right. easy.
-           right.
-           apply IHc. easy. easy.
-           subst. simpl in H. easy.
-       - case_eq d; intros.
-         + subst. simpl in H. easy.
-         + subst. simpl in H. easy. 
-         + subst. simpl in H. simpl.
-           apply IHc. easy.
-           simpl in H0. easy.
-Qed.
-
-Lemma helper1: forall c d n s, refCtxT c d -> memT n s c -> memT n s d.
-Proof. intro c.
-       induction c; intros.
-       - case_eq d; intros.
-         + subst. simpl in H0. easy.
-         + subst. simpl in H0. easy.
-         + subst. simpl in H0. easy.
-       - case_eq d; intros.
-         + subst. simpl in H. easy.
-         + subst. simpl in H. simpl.
-           apply IHc. easy. easy.
-           subst. simpl in H. easy.
-       - case_eq d; intros.
-         + subst. simpl in H. easy.
-         + subst. simpl in H. easy.
-         + subst. simpl in H. simpl.
-           simpl in H0.
-           destruct H0.
-           destruct H0.
-           subst. 
-           destruct H1. left.
-           split. easy.
-           destruct H. destruct H. destruct H2.
-           subst. left.
-           specialize (stTrans s l l0 H0 H2); intro HT. easy.
-           subst. left. easy.
-           subst. left.
-           destruct H.
-           destruct H. split. easy.
-           destruct H1. left. easy. right. easy.
-           right.
-           apply IHc. easy. easy.
-Qed.
-
-Lemma helper: forall c c' u, refCtxT c c' -> eq_ctxL u c -> eq_ctxL u c'. 
-Proof. intro c.
-       induction c; intros.
-       - case_eq c'; intros.
-         + subst. easy.
-         + subst. simpl in H. easy.
-         + subst. simpl in H. easy.
-       - case_eq c'; intros.
-         + subst. simpl in H. easy.
-         + subst. simpl in H.
-           destruct H as ((Ha1,Ha2),Hb).
-           unfold eq_ctxL in H0.
-           unfold eq_ctxL.
-           split. 
-           intros.
-           apply H0 in H. simpl in H.
-           simpl.
-           destruct H. left. subst.
-           split. easy. 
-           destruct Ha2.
-           destruct H. destruct H2.
-           left.
-           apply sstrans with (s2 := s); easy.
-           subst. left. easy.
-           subst. easy.
-           right. 
-           apply helper0 with (c := c); easy.
-           intros.
-           apply H0 in H. simpl in H.
-           simpl.  
-           apply helper1 with (c := c); easy.
-           subst. simpl in H. easy.
-       - case_eq c'; intros.
-         + subst. simpl in H. easy.
-         + subst. simpl in H. easy.
-         + subst. simpl in H.
-           destruct H as ((Ha1,Ha2),Hb).
-           unfold eq_ctxL in H0.
-           unfold eq_ctxL.
-           split. 
-           intros.
-           apply H0 in H. simpl in H.
-           simpl.
-           apply helper0 with (c := c); easy.
-           intros. 
-           apply H0 in H. simpl in H.
-           destruct H. left. subst.
-           split. easy. 
-           destruct Ha2.
-           destruct H. destruct H2.
-           left.
-           specialize (stTrans t l l0 H2 H1); intro HT. easy.
-           subst. left. easy.
-           subst. easy.
-           right.
-           apply helper1 with (c := c); easy.
-Qed.
-
-
-Lemma _a23_e: forall P (n: fin) m em n T G,
-  typ_proc m em G P T ->
-  (P = (p_var n) -> exists T' G', eq_ctxL (extendT G' n T') G /\ subtypeC T' T).
-Proof. intros.
-       induction H; intros; try easy.
-       inversion H0. subst.
-       induction c; intros.
-       simpl in H. easy.
-       simpl in H.
-       specialize(IHc H).
-       destruct IHc as (T',(G',(Ha,Hb))).
-       exists  T'. exists (consS n1 s G').
-
-       split.
-       unfold extendT.
-       unfold eq_ctxL in *. 
-       split.
-       intros n2 s0 HH. simpl.
-       destruct Ha as (Ha1,Ha2).
-
-       destruct HH as [HH | HH].
-       destruct HH as( H1a, H1b).
-       destruct H1b as [HH | HH].
-       subst. unfold extendT. simpl.
-       left. split. easy. left. easy.
-       left. split. easy.
-       right. easy.
-       right.
-       apply Ha1. easy.
-       
-       intros.
-       simpl. simpl in H1.
- 
-       destruct Ha as (Ha,Hc).
-       apply Hc in H1.
-       simpl in H1. easy.
-       easy.
-
-(*        intro HH.
-       simpl in HH.
-       destruct HH as [HH | HH].
-       destruct HH as( H1a, H1b).
-       destruct H1b as [HH | HH].
-       subst. unfold extendT. simpl.
-       left. split. easy. left. easy.
-       left. split. easy.
-       right. easy.
-       right.
-       apply Ha1. easy. *)
-
-(*        intros.
-       destruct Ha as (Ha1,Ha2).
-       split. intro HH.
-       simpl in HH. simpl.
-       apply Ha2 in HH.
-       unfold extendT in HH. simpl in HH. easy.
-       intro HH.
-       simpl. simpl in HH.
-       apply Ha2. simpl. easy.
-       easy. *)
-
-       simpl in H.
-       case_eq((Nat.eqb n0 n1)); intro Heq.
-       rewrite Heq in H. inversion H. subst.
-       exists l. exists c. split. unfold extendT.
-       apply Nat.eqb_eq in Heq. subst. easy.
-       specialize(stRefl l); intro HT. easy.
-       rewrite Heq in H.
-       specialize(IHc H).
-       destruct IHc as (T',(G',(Ha,Hb))).
-       exists T'. exists (consT n1 l G').
-       split.
-
-       unfold eq_ctxL, extendT in *.
-       split.
-       intros. simpl.
-       destruct Ha as (Ha1,Ha2).
-(*        split. intro HH. *)
-       apply Ha1. easy.
-       intros. simpl. simpl in H1.
-       
-       destruct H1.
-       right. apply Ha.
-       simpl. left. easy.
-       destruct H1.
-       left. easy.
-       right.
-       apply Ha. simpl. right. easy.
-       easy.
-
-       specialize(IHtyp_proc H0).
-       destruct IHtyp_proc as (T',(G',(Ha,Hb))).
-       exists T'. exists G'.
-       split.
-       apply helper with (c := c); easy.
-       specialize(stTrans T' t t' Hb H1); intro HT. easy.
-Qed.
-
-Lemma _a23_f: forall P m em T G,
-  typ_proc m em G P T ->
-  (P = (p_inact) -> T = ltt_end).
-Proof. intros.
-       induction H; intros; try easy.
-       subst. 
-       specialize(IHtyp_proc eq_refl).
-       subst.
-       punfold H1. inversion H1. easy.
-       apply st_mon.
-Qed.
 
 Lemma _a21: forall P Q m em T G,
   typ_proc m em G Q T ->
-  typ_proc (S m) em (extendT G m T) P T ->
-  typ_proc m em G (subst_proc Q P) T.
+  typ_proc (S m) em (extendT G m T) P T.
+(*   typ_proc m em G (subst_proc Q P) T. *)
 Proof. Admitted.
-
 
 
 
