process/typecheck_examples.v
@@ -5,15 +5,76 @@ From mathcomp Require Import ssreflect.seq.
 Import ListNotations.
 From Paco Require Import paco.
 
+Definition PBob: process := p_recv "Alice" [(1, p_send "Carol" 2 (e_val (vnat 100)) p_inact);
+                                            (4, p_send "Carol" 2 (e_val (vnat 2)) p_inact)].
 
-Definition PG_agency : process := p_rec (p_recv "Customer" [(0, sbool, p_send "Customer" 1 (e_val (vnat 5000)) (p_recv "Customer" [
-  (2, sbool, p_recv "Customer" [(3, snat, (p_send "Customer" 4 (e_val (vnat 25122019)) p_inact))]);
-  (5, sbool, p_rec (p_var 0));
-  (6, sbool, p_inact)]));
-        (7, sbool, p_send "Customer" 1 (e_val (vnat 1000)) (p_recv "Customer" [
-  (2, sbool, p_recv "Customer" [(3, snat, (p_send "Customer" 4 (e_val (vnat 25122019)) p_inact))]);
-  (5, sbool, p_rec (p_var 0));
-  (6, sbool, p_inact)]))
+Definition TBob: ltt := ltt_recv "Alice" [(1, snat, ltt_send "Carol" [(2, snat, ltt_end)]);
+                                          (4, snat, ltt_send "Carol" [(2, snat, ltt_end)])].
+
+Example _317_b: typ_proc 0 emptyS emptyT PBob TBob.
+Proof. unfold PBob, TBob.
+       (* typechecking the outermost structure *)
+       specialize(tc_recv 0 emptyS emptyT "Alice"
+                         [1; 4]
+                         [snat; snat]
+                         [(p_send "Carol" 2 (e_val (vnat 100)) p_inact); (p_send "Carol" 2 (e_val (vnat 2)) p_inact)]
+                         [(ltt_send "Carol" [(2, snat, ltt_end)]); (ltt_send "Carol" [(2, snat, ltt_end)])]
+                         ); intro HR.
+       simpl in HR.
+       apply HR; clear HR; try easy.
+       apply Forall_forall.
+       intros (s, (p, l)) HIn.
+       simpl in HIn.
+       destruct HIn as [HIn | HIn].
+       inversion HIn. simpl.
+       subst.
+
+       (* typechecking the first continuation *)
+       specialize(tc_send 1 (extendS emptyS 0 snat) emptyT "Carol"
+                          2
+                          (e_val (vnat 100))
+                          p_inact
+                          snat
+                          ltt_end
+         ); intro HS.
+       simpl in HS.
+       apply HS; clear HS.
+
+       (*expression typcheck*)
+       constructor.
+
+       constructor.
+       simpl.
+       destruct HIn as [HIn | HIn].
+       inversion HIn. simpl.
+       subst.
+       (* typechecking the second continuation *)
+       specialize(tc_send 1 (extendS emptyS 0 snat) emptyT "Carol"
+                          2
+                          (e_val (vnat 2))
+                          p_inact
+                          snat
+                          ltt_end
+         ); intro HS.
+       simpl in HS.
+       apply HS; clear HS.
+
+       (*expression typcheck*)
+       constructor.
+
+       constructor.
+
+       easy.
+Qed.
+
+Definition PG_agency : process := p_rec 0 (p_recv "Customer" [(0, p_send "Customer" 1 (e_val (vnat 5000)) (p_recv "Customer" [
+  (2, p_recv "Customer" [(3, (p_send "Customer" 4 (e_val (vnat 25122019)) p_inact))]);
+  (5, p_var 0);
+  (6, p_inact)]));
+        (7, p_send "Customer" 1 (e_val (vnat 1000)) (p_recv "Customer" [
+  (2, p_recv "Customer" [(3, (p_send "Customer" 4 (e_val (vnat 25122019)) p_inact))]);
+  (5, p_var 0);
+  (6, p_inact)]))
   ]).
 
 CoFixpoint TG_agency : ltt := ltt_recv "Customer" [(0, sbool, ltt_send "Customer" [(1, snat, ltt_recv "Customer" [
@@ -25,12 +86,11 @@ CoFixpoint TG_agency : ltt := ltt_recv "Customer" [(0, sbool, ltt_send "Customer
   (5, sbool, TG_agency);
   (6, sbool, ltt_end)])])].
 
-Example _vgi_agency_ : typ_proc 0 0 empty PG_agency TG_agency.
+Example _vgi_agency_ : typ_proc 0 emptyS emptyT PG_agency TG_agency.
 Proof. unfold PG_agency.
   rewrite(ltt_eq TG_agency). simpl.
   constructor.
-  
-  specialize(tc_recv 1 0 (extendT empty 0
+  specialize(tc_recv 0 emptyS (extendT emptyT 0
   (ltt_recv "Customer" [
     (0, sbool,
       ltt_send "Customer" [(1, snat,
@@ -48,17 +108,17 @@ Proof. unfold PG_agency.
   [0; 7] 
   [sbool; sbool]
   [p_send "Customer" 1 (e_val (vnat 5000)) (
-    p_recv "Customer" [(2, sbool, 
-    p_recv "Customer" [(3, snat, (
+    p_recv "Customer" [(2, 
+    p_recv "Customer" [(3, (
     p_send "Customer" 4 (e_val (vnat 25122019)) p_inact))]);
-    (5, sbool, p_rec (p_var 0));
-    (6, sbool, p_inact)]);
+    (5, p_var 0);
+    (6, p_inact)]);
   p_send "Customer" 1 (e_val (vnat 1000)) (
-    p_recv "Customer" [(2, sbool, 
-    p_recv "Customer" [(3, snat, (
+    p_recv "Customer" [(2,  
+    p_recv "Customer" [(3,  (
     p_send "Customer" 4 (e_val (vnat 25122019)) p_inact))]);
-    (5, sbool, p_rec (p_var 0));
-    (6, sbool, p_inact)])
+    (5, p_var 0);
+    (6, p_inact)])
   ]
   [ltt_send "Customer" [(1, snat, ltt_recv "Customer" [
   (2, sbool, ltt_recv "Customer" [(3, snat, ltt_send "Customer" [(4, snat, ltt_end)])]);
@@ -80,26 +140,26 @@ Proof. unfold PG_agency.
   subst.
   constructor.
   constructor.
-  specialize(tc_recv 1 1 (extendS
-     (extendT empty 0
-        (ltt_recv "Customer"
-           [(0, sbool,
-             ltt_send "Customer"
-               [(1, snat,
-                 ltt_recv "Customer"
-                   [(2, sbool, ltt_recv "Customer" [(3, snat, ltt_send "Customer" [(4, snat, ltt_end)])]);
-                    (5, sbool, TG_agency); (6, sbool, ltt_end)])]);
-            (7, sbool,
-             ltt_send "Customer"
-               [(1, snat,
-                 ltt_recv "Customer"
-                   [(2, sbool, ltt_recv "Customer" [(3, snat, ltt_send "Customer" [(4, snat, ltt_end)])]);
-                    (5, sbool, TG_agency); (6, sbool, ltt_end)])])])) 0 sbool) "Customer"
+  specialize(tc_recv 1 (extendS emptyS 0 sbool)
+     (extendT emptyT 0
+     (ltt_recv "Customer"
+        [(0, sbool,
+          ltt_send "Customer"
+            [(1, snat,
+              ltt_recv "Customer"
+                [(2, sbool, ltt_recv "Customer" [(3, snat, ltt_send "Customer" [(4, snat, ltt_end)])]);
+                 (5, sbool, TG_agency); (6, sbool, ltt_end)])]);
+         (7, sbool,
+          ltt_send "Customer"
+            [(1, snat,
+              ltt_recv "Customer"
+                [(2, sbool, ltt_recv "Customer" [(3, snat, ltt_send "Customer" [(4, snat, ltt_end)])]);
+                 (5, sbool, TG_agency); (6, sbool, ltt_end)])])])) "Customer"
       [2; 5; 6]
       [sbool; sbool; sbool]
       [
-        p_recv "Customer" [(3, snat, p_send "Customer" 4 (e_val (vnat 25122019)) p_inact)];
-        p_rec (p_var 0);
+        p_recv "Customer" [(3, p_send "Customer" 4 (e_val (vnat 25122019)) p_inact)];
+        p_var 0;
         p_inact
       ]
       [
@@ -113,24 +173,21 @@ Proof. unfold PG_agency.
   intros (s, (p, l)) HI1. simpl in HI1.
   destruct HI1 as [HI1 | HI2].
   inversion HI1. simpl. subst.
-  specialize(tc_recv 1 2 (extendS
-     (extendS
-        (extendT empty 0
-           (ltt_recv "Customer"
-              [(0, sbool,
-                ltt_send "Customer"
-                  [(1, snat,
-                    ltt_recv "Customer"
-                      [(2, sbool,
-                        ltt_recv "Customer" [(3, snat, ltt_send "Customer" [(4, snat, ltt_end)])]);
-                       (5, sbool, TG_agency); (6, sbool, ltt_end)])]);
-               (7, sbool,
-                ltt_send "Customer"
-                  [(1, snat,
-                    ltt_recv "Customer"
-                      [(2, sbool,
-                        ltt_recv "Customer" [(3, snat, ltt_send "Customer" [(4, snat, ltt_end)])]);
-                       (5, sbool, TG_agency); (6, sbool, ltt_end)])])])) 0 sbool) 1 sbool) "Customer"
+  specialize(tc_recv 2 (extendS (extendS emptyS 0 sbool) 1 sbool)
+     (extendT emptyT 0
+     (ltt_recv "Customer"
+        [(0, sbool,
+          ltt_send "Customer"
+            [(1, snat,
+              ltt_recv "Customer"
+                [(2, sbool, ltt_recv "Customer" [(3, snat, ltt_send "Customer" [(4, snat, ltt_end)])]);
+                 (5, sbool, TG_agency); (6, sbool, ltt_end)])]);
+         (7, sbool,
+          ltt_send "Customer"
+            [(1, snat,
+              ltt_recv "Customer"
+                [(2, sbool, ltt_recv "Customer" [(3, snat, ltt_send "Customer" [(4, snat, ltt_end)])]);
+                 (5, sbool, TG_agency); (6, sbool, ltt_end)])])])) "Customer"
         [3] [snat] [p_send "Customer" 4 (e_val (vnat 25122019)) p_inact] [ltt_send "Customer" [(4, snat, ltt_end)]]
   ); intro HR. simpl in HR. apply HR.
   try easy. try easy. try easy. simpl. clear HR. 
@@ -144,8 +201,9 @@ Proof. unfold PG_agency.
   inversion HI3.
   destruct HI2 as [HI2 | HI3].
   inversion HI2. subst.
-  constructor. constructor. simpl.
-  rewrite (ltt_eq TG_agency) at 1. simpl. try easy.
+  simpl. 
+  apply tc_var. simpl.
+  rewrite (ltt_eq TG_agency) at 1. simpl. easy.
   destruct HI3 as [HI3 | HI4].
   inversion HI3. subst. 
   constructor.
@@ -153,26 +211,26 @@ Proof. unfold PG_agency.
   destruct HI1 as [HI1 | HI2].
   inversion HI1. simpl. subst.
   constructor. constructor. 
-  specialize(tc_recv 1 1 (extendS
-     (extendT empty 0
-        (ltt_recv "Customer"
-           [(0, sbool,
-             ltt_send "Customer"  
-               [(1, snat,
-                 ltt_recv "Customer"
-                   [(2, sbool, ltt_recv "Customer" [(3, snat, ltt_send "Customer" [(4, snat, ltt_end)])]);
-                    (5, sbool, TG_agency); (6, sbool, ltt_end)])]);
-            (7, sbool,
-             ltt_send "Customer"
-               [(1, snat,
-                 ltt_recv "Customer"
-                   [(2, sbool, ltt_recv "Customer" [(3, snat, ltt_send "Customer" [(4, snat, ltt_end)])]);
-                    (5, sbool, TG_agency); (6, sbool, ltt_end)])])])) 0 sbool) "Customer"
+  specialize(tc_recv 1 (extendS emptyS 0 sbool)
+     (extendT emptyT 0
+     (ltt_recv "Customer"
+        [(0, sbool,
+          ltt_send "Customer"
+            [(1, snat,
+              ltt_recv "Customer"
+                [(2, sbool, ltt_recv "Customer" [(3, snat, ltt_send "Customer" [(4, snat, ltt_end)])]);
+                 (5, sbool, TG_agency); (6, sbool, ltt_end)])]);
+         (7, sbool,
+          ltt_send "Customer"
+            [(1, snat,
+              ltt_recv "Customer"
+                [(2, sbool, ltt_recv "Customer" [(3, snat, ltt_send "Customer" [(4, snat, ltt_end)])]);
+                 (5, sbool, TG_agency); (6, sbool, ltt_end)])])])) "Customer"
       [2; 5; 6]
       [sbool; sbool; sbool]
       [
-        p_recv "Customer" [(3, snat, p_send "Customer" 4 (e_val (vnat 25122019)) p_inact)];
-        p_rec (p_var 0);
+        p_recv "Customer" [(3, p_send "Customer" 4 (e_val (vnat 25122019)) p_inact)];
+        p_var 0;
         p_inact
       ]
       [
@@ -186,24 +244,21 @@ Proof. unfold PG_agency.
   intros (s, (p, l)) HI4. simpl in HI4.
   destruct HI4 as [HI4 | HI5].
   inversion HI4. simpl. subst.
-  specialize(tc_recv 1 2 (extendS
-     (extendS
-        (extendT empty 0
-           (ltt_recv "Customer"
-              [(0, sbool,
-                ltt_send "Customer"
-                  [(1, snat,
-                    ltt_recv "Customer"
-                      [(2, sbool,
-                        ltt_recv "Customer" [(3, snat, ltt_send "Customer" [(4, snat, ltt_end)])]);
-                       (5, sbool, TG_agency); (6, sbool, ltt_end)])]);
-               (7, sbool,
-                ltt_send "Customer"
-                  [(1, snat,
-                    ltt_recv "Customer"
-                      [(2, sbool,
-                        ltt_recv "Customer" [(3, snat, ltt_send "Customer" [(4, snat, ltt_end)])]);
-                       (5, sbool, TG_agency); (6, sbool, ltt_end)])])])) 0 sbool) 1 sbool) "Customer"
+  specialize(tc_recv 2 (extendS (extendS emptyS 0 sbool) 1 sbool)
+     (extendT emptyT 0
+     (ltt_recv "Customer"
+        [(0, sbool,
+          ltt_send "Customer"
+            [(1, snat,
+              ltt_recv "Customer"
+                [(2, sbool, ltt_recv "Customer" [(3, snat, ltt_send "Customer" [(4, snat, ltt_end)])]);
+                 (5, sbool, TG_agency); (6, sbool, ltt_end)])]);
+         (7, sbool,
+          ltt_send "Customer"
+            [(1, snat,
+              ltt_recv "Customer"
+                [(2, sbool, ltt_recv "Customer" [(3, snat, ltt_send "Customer" [(4, snat, ltt_end)])]);
+                 (5, sbool, TG_agency); (6, sbool, ltt_end)])])])) "Customer"
         [3] [snat] [p_send "Customer" 4 (e_val (vnat 25122019)) p_inact] [ltt_send "Customer" [(4, snat, ltt_end)]]
   ); intro HR. simpl in HR. apply HR.
   try easy. try easy. try easy. simpl. clear HR. 
@@ -217,19 +272,19 @@ Proof. unfold PG_agency.
   inversion HI6.
   destruct HI5 as [HI5 | HI6].
   inversion HI5. simpl. subst. 
-  constructor. constructor. simpl. 
+  constructor. simpl.
   rewrite (ltt_eq TG_agency) at 1. simpl. try easy.
   destruct HI6 as [HI6 | HI7].
   inversion HI6. subst. simpl. constructor.
   inversion HI7. inversion HI2.
 
-Qed.
+Qed. 
 
 
-Definition PBob2: process := p_rec (p_send "Carol" 2 (e_val (vnat 100)) (p_var 0)).
+Definition PBob2: process := p_rec 0 (p_send "Carol" 2 (e_val (vnat 100)) (p_var 0)).
 CoFixpoint TBob2: ltt := ltt_send "Carol" [(2, snat, TBob2)].
 
-Example newEx: typ_proc 0 0 empty PBob2 TBob2.
+Example newEx: typ_proc 0 emptyS emptyT PBob2 TBob2.
 Proof. unfold PBob2.
        rewrite(ltt_eq TBob2). simpl.
        constructor.
@@ -242,21 +297,20 @@ Proof. unfold PBob2.
 Qed.
 
 
-Definition PTestmu : process := p_rec (p_recv "A" [(0, sbool, p_inact)]).
+Definition PTestmu : process := p_rec 0 (p_recv "A" [(0, p_inact)]).
 Definition TTestmu : ltt := ltt_recv "A" [(0, sbool, ltt_end)].
 
-Example _testmu_1 : typ_proc 0 0 empty PTestmu TTestmu.
+Example _testmu_1 : typ_proc 0 emptyS emptyT PTestmu TTestmu.
 Proof. 
   unfold PTestmu, TTestmu.
-  specialize(tc_mu 0 0 empty (p_recv "A" [(0, sbool, p_inact)]) (ltt_recv "A" [(0, sbool, ltt_end)])). intro HR.
-  apply HR. clear HR.
-  specialize(tc_recv 1 0 (extendT empty 0 (ltt_recv "A" [(0, sbool, ltt_end)])) "A"
+  constructor.
+  specialize(tc_recv 0 emptyS (extendT emptyT 0 (ltt_recv "A" [(0, sbool, ltt_end)])) "A"
     [0] [sbool] [p_inact] [ltt_end]
   ); intro HR.
   simpl in HR. simpl. apply HR. clear HR. 
-  try easy. clear HR. 
-  try easy. clear HR.
-  try easy. clear HR.
+  try easy; clear HR. 
+  try easy; clear HR.
+  try easy; clear HR.
   apply Forall_forall.
   intros (s, (p, l)) HIn.
   simpl in HIn. 
@@ -268,13 +322,12 @@ Qed.
 
 
 
-  
-Example pr3 : process := p_rec (p_recv "Alice" [
-  (0, sbool, p_var 0);
-  (1, sbool, p_rec (p_recv "Bob" [
-    (2, sbool, p_var 0);
-    (3, sbool, p_var 1);
-    (4, sbool, p_inact)
+Example pr3 : process := p_rec 0 (p_recv "Alice" [
+  (0, p_var 0);
+  (1, p_rec 1 (p_recv "Bob" [
+    (2, p_var 0);
+    (3, p_var 1);
+    (4, p_inact)
     ]))
   ]).
   
