process/inversion.v
@@ -1,0 +1,332 @@
+From SST Require Import aux.unscoped aux.expressions process.processes process.typecheck type.global tree.global tree.local.
+Require Import List String Datatypes ZArith Relations PeanoNat.
+Open Scope list_scope.
+From mathcomp Require Import ssreflect.seq.
+Import ListNotations.
+From Paco Require Import paco.
+
+Lemma zip_eq: forall {A B: Type} (l1 l3: list A) (l2 l4: list B),
+  length l1 = length l2 -> length l2 = length l3 -> length l3 = length l4 ->
+  (zip l1 l2) = (zip l3 l4) ->
+  l1 = l3 /\ l2 = l4.
+Proof. intros A B l1.
+       induction l1; intros.
+       - simpl in *.
+         rewrite <- H in H0.
+         rewrite <- H0 in H1.
+         rewrite empty_nil in H.
+         rewrite empty_nil in H0.
+         rewrite empty_nil in H1.
+         subst. easy.
+       - simpl in H.
+         case_eq l2; intros.
+         + subst. simpl in *. easy.
+         + subst. simpl in *.
+           case_eq l3; intros.
+           ++ subst. easy.
+           ++ case_eq l4; intros.
+              -- subst. easy.
+              -- subst. simpl in *.
+                 inversion H2. subst.
+                 inversion H.
+                 inversion H1.
+                 inversion H0.
+                 specialize(IHl1 l0 l l2 H4 H7 H5 H6).
+                 split. f_equal. easy.
+                 f_equal. easy.
+Qed.
+
+Lemma zip_len: forall {A B: Type} (l1: list A) (l2: list B),
+  length l1 = length l2 -> length l1 = length (zip l1 l2).
+Proof. intros A B l1.
+       induction l1; intros.
+       - simpl in H. rewrite empty_nil in H.
+         subst. simpl. easy.
+       - simpl in H. simpl.
+         case_eq l2; intros.
+         subst. easy.
+         subst. simpl in H.
+         inversion H.
+         simpl. f_equal.
+         apply IHl1. easy.
+Qed.
+
+Lemma _a23_a: forall em p L Q P Gs Gt T, 
+  typ_proc em Gs Gt P T ->
+  P = (p_recv p (zip L Q)) -> 
+  (exists T' S, length T' = length L -> length T' = length S -> length T' = length Q -> subtypeC (ltt_recv p (zip (zip L S) T')) T /\  
+  List.Forall (fun u => typ_proc (Datatypes.S em) (extendS Gs em (fst u)) Gt (fst (snd u)) (snd (snd u))) (zip S (zip Q T'))).
+Proof. intros.
+       induction H; intros; try easy.
+       specialize(IHtyp_proc H0).
+       destruct IHtyp_proc as (T',IHtyp_proc).
+       exists T'.
+       simpl.
+       destruct IHtyp_proc as [S'].
+       exists S'.
+       intros Hla1 Hla2 Hla3.
+       split.
+       specialize(H4 Hla1 Hla2 Hla3).
+       destruct H4 as (IHtyp_proc, Ha).
+       specialize(stTrans (ltt_recv p (zip (zip L S') T')) t t' IHtyp_proc); intro HT.
+       apply HT.
+       easy.
+       
+       (**)
+       destruct H4 as (IHtyp_proc, Ha). easy. easy. easy.
+       apply Forall_forall.
+       intros (x1,(x2,x3)) Hx.
+       simpl in *.
+       rewrite Forall_forall in Ha.
+       specialize(Ha (x1,(x2,x3))). simpl in Ha.
+       specialize(tc_sub (Datatypes.S em) (extendS cs em x1) (extendS cs' em x1) ct ct' x2 x3 x3); intro HTC.
+       apply HTC.
+(*        specialize(tc_sub m (Datatypes.S em) c); intro HTC. *)
+       apply Ha. easy.
+       apply stRefl.
+       simpl.
+       split. split. split. right. easy. easy. easy.
+
+       rewrite Forall_forall in H3.
+       exists T. exists ST.
+       intros Hla1 Hla2 Hla3.
+       split.
+       inversion H0. subst.
+       assert(length (zip L0 ST) = length L0) as Hasrt1.
+       { symmetry.
+         apply zip_len. easy.
+       }
+       assert(L0 = L /\ P = Q).
+       { 
+          specialize(eq_trans H H1); intros.
+          specialize(eq_trans H2 Hla1); intros.
+          specialize(eq_trans (eq_sym Hla1) Hla3); intros.
+          specialize(zip_eq L0 L P Q H4 H5 H7 H6); intros.
+          easy.
+       }
+       subst.
+       pfold.
+       destruct H4.
+       replace L0 with L.
+       apply sub_in. easy. easy.
+       clear H H1 H2 H3 H6 Hla1 Hla2 Hla3 Hasrt1.
+       apply Forall_forall.
+       intros (x1,x2) Hx.
+       induction ST; intros.
+       simpl in Hx. easy.
+       simpl in Hx.
+       destruct Hx as [Hx | Hx].
+       inversion Hx. subst.
+       simpl. apply srefl.
+       simpl. apply IHST. easy. 
+
+       apply Forall_forall.
+       intros (x1,x2) Hx.
+       clear H H1 H2 H3 Hla1 Hla2 Hla3 Hasrt1.
+       induction T; intros.
+       simpl in Hx. easy.
+       simpl in Hx.
+       simpl in IHT.
+       destruct Hx as [Hx | Hx].
+       inversion Hx. subst. simpl.
+       specialize(stRefl x2); intro HT.
+       punfold HT. apply st_mon.
+       simpl. apply IHT. easy.
+       
+       (**)
+       apply Forall_forall.
+       intros (x1,(x2,x3)) Hx.
+       simpl in *.
+       specialize(H3 (x1,(x2,x3))). simpl in H3.
+       inversion H0. subst.
+       apply H3.
+       assert(L0 = L /\ P = Q).
+       { 
+          specialize(eq_trans H H1); intros.
+          specialize(eq_trans H2 Hla1); intros.
+          specialize(eq_trans (eq_sym Hla1) Hla3); intros.
+          specialize(zip_eq L0 L P Q H4 H5 H7 H6); intros.
+          easy.
+       }
+       destruct H4.
+       subst.
+       easy.
+Qed.
+
+
+Lemma _a23_b: forall em p l e Q P Gs Gt T, 
+  typ_proc em Gs Gt P T ->
+  P = (p_send p l e Q) -> exists S S' T', typ_expr Gs e S /\ typ_proc em Gs Gt Q T' /\ subsort S' S /\ subtypeC (ltt_send p [(l,S',T')]) T.
+Proof. intros em p l e Q P Gs Gt T H.
+       induction H; intros; try easy.
+       specialize(IHtyp_proc H3).
+       destruct IHtyp_proc as (S,(S',(T',Ha))).
+       exists S. exists S'. exists T'.
+       split.
+       specialize(sc_sub cs cs' e S S); intro HSS.
+       apply HSS. easy. apply srefl. easy.
+       split.
+       specialize(tc_sub em cs cs' ct ct' Q T' T'); intro HTS.
+       apply HTS. easy.
+       apply stRefl. easy. easy. split. easy.
+       destruct Ha as (Ha,(Hb,(Hc,Hd))).
+       specialize(stTrans (ltt_send p [(l, S', T')]) t t' Hd H0); intro HT.
+       apply HT.
+       exists S. exists S. exists T.
+       inversion H1. subst.
+       split. easy. split. easy.
+       split. apply srefl. 
+       specialize(sub_out (upaco2 subtype bot2)
+          p [l] [S] [S] [T] [T]
+        ); intros HHa.
+       simpl in HHa.
+       pfold.
+       apply HHa. easy. easy.
+       apply Forall_forall. simpl.
+       intros (s1, s2) Hs. destruct Hs.
+       inversion H2. subst. simpl. apply srefl.
+       easy.
+       apply Forall_forall. simpl.
+       intros (T1, T2) Hs. destruct Hs.
+       inversion H2. subst.
+       simpl. left. pfold.
+       specialize(stRefl T2); intro HT.
+       punfold HT. apply st_mon.
+       easy.
+Qed.
+
+Lemma _a23_c: forall P em e Q1 Q2 T Gs Gt,
+  typ_proc em Gs Gt P T ->
+  P = (p_ite e Q1 Q2) -> exists T1 T2, typ_proc em Gs Gt Q1 T1 /\ typ_proc em Gs Gt Q2 T2 /\ subtypeC T1 T /\ subtypeC T2 T.
+Proof. intros.
+       induction H; intros; try easy.
+       inversion H0.
+       subst.
+       exists T. exists T.
+       split. easy. split. easy. split. easy. easy.
+       
+       specialize(IHtyp_proc H0).
+       destruct IHtyp_proc as (T1,(T2,(Ha,(Hb,(Hc,Hd))))).
+       exists T1. exists T2.
+       split.
+       specialize(tc_sub em cs cs' ct ct' Q1 T1 T1); intro HTS.
+       apply HTS. easy. apply stRefl. easy. easy.
+       split.
+       specialize(tc_sub em cs cs' ct ct' Q2 T2 T2); intro HTS.
+       apply HTS. easy. apply stRefl. easy. easy. 
+       split.
+       specialize(stTrans T1 t t' Hc H1); intro HT. easy.
+       specialize(stTrans T2 t t' Hd H1); intro HT. easy.
+Qed.
+
+Lemma _a23_d: forall P em x Q T Gs Gt,
+  typ_proc em Gs Gt P T ->
+  P = (p_rec x Q)   -> typ_proc em Gs (extendT Gt x T) Q T.
+Proof. intros.
+       induction H; intros; try easy.
+       inversion H0. subst.
+       unfold ct' in *. easy.
+
+       subst.
+       apply tc_sub with
+       (ct := extendT ct x t) (cs := cs) (t := t).
+       apply IHtyp_proc. easy.
+       easy. easy.
+       split. split. split. left. easy. easy.
+Qed.
+
+Lemma helper_a23_e_1 : forall x X n l x0 ct t, (Some t = lookupT ct X) -> (leq_ctxT (extendT x0 X x) ct) -> ((X =? n)%nat = false)
+    -> subtypeC x t -> leq_ctxT (consT X x (consT n l x0)) (consT n l ct).
+Proof. 
+  unfold leq_ctxT at 2. unfold leq_tinctx_prop.
+  induction lookupT; intros; try easy.
+  
+  case_eq (Nat.eqb n0 X); intros; try easy.
+  specialize(natb_to_prop n0 X H3); intros. subst. simpl.
+  replace (X =? X)%nat with true.
+  replace (X =? n)%nat with false.
+  replace (lookupT ct X) with (Some t).
+  easy.
+  
+  simpl. 
+  replace (n0 =? X)%nat with false.
+  case_eq (Nat.eqb n0 n); intros; try easy.
+  unfold leq_ctxT in H0. unfold leq_tinctx_prop in H0.
+  specialize(H0 n0). simpl in H0.
+  replace (n0 =? X)%nat with false in H0. easy.
+  
+  case_eq (Nat.eqb n0 X); intros; try easy.
+  specialize(natb_to_prop n0 X H3); intros. subst. simpl.
+  replace (X =? X)%nat with true.
+  replace (X =? n)%nat with false.
+  replace (lookupT ct X) with (Some t).
+  easy.
+  
+  simpl. 
+  replace (n0 =? X)%nat with false.
+  case_eq (Nat.eqb n0 n); intros; try easy.
+  unfold leq_ctxT in H0. unfold leq_tinctx_prop in H0.
+  specialize(H0 n0). simpl in H0.
+  replace (n0 =? X)%nat with false in H0. easy.
+  
+  apply emptyT.
+  apply 0.
+  
+Qed.
+
+Lemma _a23_e: forall P em X T Gs Gt,
+  typ_proc em Gs Gt P T ->
+  (P = (p_var X) -> exists T' G', leq_ctxT (extendT G' X T') Gt /\ subtypeC T' T).
+Proof. intros.
+       induction H; intros; try easy.
+       inversion H0. subst.
+       induction ct; intros. easy.
+       simpl in H.
+       
+       case_eq (Nat.eqb X n); intros Hb.
+       
+       replace (X =? n)%nat with true in H.
+       inversion H. 
+       exists l. exists ct. unfold extendT. 
+       split. 
+       specialize(natb_to_prop X n Hb); intros.
+       subst.
+       apply leq_ctxT_refl.
+       easy.
+
+       replace (X =? n)%nat with false in H.
+       specialize(IHct H).
+       destruct IHct. destruct H1.
+       exists x. exists (consT n l x0).
+       split. unfold extendT.
+       destruct H1.
+       specialize(helper_a23_e_1 x X n l x0 ct t H H1 Hb H2); intros.
+       easy.
+       
+       destruct H1.
+       easy.
+       
+       specialize(IHtyp_proc H0).
+       destruct IHtyp_proc. destruct H4.
+       specialize(ref_stronger_T ct ct' H3); intros.
+       destruct H4.
+       specialize(leq_ctxT_trans (extendT x0 X x) ct ct' H4 H5); intros.
+       specialize(stTrans x t t' H6 H1); intros.
+       exists x. exists x0.
+       split.
+       apply H7.
+       apply H8.
+      
+Qed.
+
+Lemma _a23_f: forall P em T Gs Gt,
+  typ_proc em Gs Gt P T ->
+  P = p_inact -> T = ltt_end.
+Proof. intros.
+       induction H; intros; try easy.
+       subst. 
+       specialize(IHtyp_proc eq_refl).
+       subst.
+       punfold H1. inversion H1. easy.
+       apply st_mon.
+Qed.
